Więcej liczb konaturalnych.

book/X8.v
@@ -1,3 +1,7 @@
+(** * X8: Liczby konaturalne *)
+
+(** TODO: coś tu napisać. *)
+
 CoInductive conat : Type :=
 {
     pred : option conat;
@@ -11,26 +15,34 @@ CoInductive sim (n m : conat) : Prop :=
         pred n = Some n' /\ pred m = Some m' /\ sim n' m'
 }.
 
+Axiom sim_eq :
+  forall n m : conat, sim n m -> n = m.
+
 Lemma sim_refl :
   forall n : conat, sim n n.
+(* begin hide *)
 Proof.
   cofix CH.
   constructor. destruct n as [[n' |]]; cbn.
     right. exists n', n'. do 2 split; try reflexivity. apply CH.
     left. do 2 constructor.
 Qed.
+(* end hide *)
 
 Lemma sim_sym :
   forall n m : conat, sim n m -> sim m n.
+(* begin hide *)
 Proof.
   cofix CH.
   constructor. destruct H as [[[] | (n' & m' & H1 & H2 & H3)]].
     auto.
     right. exists m', n'. do 2 (split; auto).
 Qed.
+(* end hide *)
 
 Lemma sim_trans :
   forall a b c : conat, sim a b -> sim b c -> sim a c.
+(* begin hide *)
 Proof.
   cofix CH.
   constructor.
@@ -40,10 +52,12 @@ Proof.
       congruence.
       exists n', x0. do 2 (try split; auto). eapply CH. eauto. congruence.
 Qed.
+(* end hide *)
 
 Require Import Setoid.
 
 Instance Equivalence_sim : Equivalence sim.
+(* begin hide *)
 Proof.
   esplit; red.
     apply sim_refl.
@@ -72,23 +86,28 @@ CoFixpoint add (n m : conat) : conat :=
 
 Lemma add_zero_l :
   forall n : conat, sim (add zero n) n.
+(* begin hide *)
 Proof.
   constructor; cbn. destruct n as [[n' |]]; cbn.
     right. exists n', n'. do 2 split; try reflexivity.
     left. auto.
 Qed.
+(* end hide *)
 
 Lemma add_zero_r :
   forall n : conat, sim (add n zero) n.
+(* begin hide *)
 Proof.
   cofix CH.
   constructor; cbn. destruct n as [[n' |]]; cbn.
     right. do 2 eexists. do 2 split; try reflexivity. apply CH.
     left. auto.
 Qed.
+(* end hide *)
 
 Lemma add_assoc :
   forall a b c : conat, sim (add (add a b) c) (add a (add b c)).
+(* begin hide *)
 Proof.
   cofix CH.
   constructor.
@@ -97,35 +116,40 @@ Proof.
     destruct b as [[|]]; cbn.
       right. do 2 eexists. do 2 split; try reflexivity. apply sim_refl.
 Qed.
+(* end hide *)
 
 Lemma add_succ_l :
   forall n m : conat, sim (add (succ n) m) (add n (succ m)).
+(* begin hide *)
 Proof.
   cofix CH.
   constructor. destruct n as [[n' |]]; cbn.
     right. do 2 eexists. do 2 split; try reflexivity. apply CH.
     right. do 2 eexists. do 2 split; try reflexivity. apply add_zero_l.
 Qed.
+(* end hide *)
 
 Lemma add_succ_r :
   forall n m : conat, sim (add n (succ m)) (add (succ n) m).
+(* begin hide *)
 Proof.
   intros. apply sim_sym, add_succ_l.
 Qed.
+(* end hide *)
 
 Ltac inv H := inversion H; subst; clear H; auto.
 
 Lemma sim_succ_succ :
   forall n m : conat, sim n m -> sim (succ n) (succ m).
+(* begin hide *)
 Proof.
   constructor. cbn. right. exists n, m. auto.
 Qed.
-
-Lemma sim_pred_pred :
-  forall n n' m m' : 
+(* end hide *)
 
 Lemma add_comm :
   forall n m : conat, sim (add n m) (add m n).
+(* begin hide *)
 Proof.
   cofix CH.
   constructor. destruct n as [[n' |]], m as [[m' |]]; cbn.
@@ -134,12 +158,124 @@ Proof.
     Focus 2. right. do 2 eexists. do 2 split; try reflexivity.
       apply sim_sym. apply add_zero_r.
     Focus 2. auto.
+    specialize (CH n' (succ m')).
     right. do 2 eexists. do 2 split; try reflexivity.
-      eapply sim_trans with (add (succ n') m').
-        rewrite add_succ_l. unfold succ. reflexivity.
-        unfold succ. apply CH.
+      rewrite (sim_eq _ _ (add_succ_l _ _)) in CH. apply CH.
 Qed.
-      
-      apply sim_trans with (add {| pred := Some m'; |} n').
-        apply CH.
-        destruct m'; cbn. Focus 2.
+(* end hide *)
+
+CoInductive le (n m : conat) : Prop :=
+{
+    le' :
+      pred n = None \/
+      exists n' m' : conat,
+        pred n = Some n' /\
+        pred m = Some m' /\ le n' m'
+}.
+
+Lemma le_refl :
+  forall n : conat, le n n.
+(* begin hide *)
+Proof.
+  cofix CH.
+  constructor. destruct n as [[n' |]]; cbn.
+    right. do 2 eexists. do 2 split; try reflexivity. apply CH.
+    left. reflexivity.
+Qed.
+(* end hide *)
+
+Lemma le_trans :
+  forall a b c : conat, le a b -> le b c -> le a c.
+(* begin hide *)
+Proof.
+  cofix CH.
+  constructor. destruct H, H0.
+  decompose [or ex and] le'0; clear le'0.
+    left. assumption.
+    decompose [or ex and] le'1; clear le'1.
+      congruence.
+      rewrite H in H3. inv H3. right. do 2 eexists. split.
+        eassumption.
+        split.
+          eassumption.
+          eapply CH; eauto.
+Qed.
+(* end hide *)
+
+Lemma le_sim :
+  forall n n' m m' : conat,
+    sim n n' -> sim m m' -> le n m -> le n' m'.
+(* begin hide *)
+Proof.
+  cofix CH.
+  constructor. destruct H1. decompose [or ex and] le'0; clear le'0.
+    left. destruct H. decompose [or and ex] sim'0.
+      assumption.
+      congruence.
+    right. exists x, x0. split; [idtac | split].
+      destruct H.
+Abort.
+(* end hide *)
+
+Lemma le_add_l :
+  forall n m : conat, le n (add n m).
+(* begin hide *)
+Proof.
+  cofix CH.
+  constructor. destruct n as [[n' |]]; cbn.
+    right. do 2 eexists. do 2 split; try reflexivity. apply CH.
+    left. reflexivity.
+Qed.
+(* end hide *)
+
+Lemma le_add_r :
+  forall n m : conat, le m (add n m).
+(* begin hide *)
+Proof.
+  cofix CH.
+  constructor. destruct n as [[n' |]], m as [[m' |]]; cbn.
+    right. do 2 eexists. do 2 split; try reflexivity.
+Abort.
+(* end hide *)
+
+Lemma le_add_l' :
+  forall n n' m : conat,
+    le n n' -> le (add n m) (add n' m).
+Proof.
+Admitted.
+
+Lemma le_add_r' :
+  forall n m m' : conat,
+    le m m' -> le (add n m) (add n m').
+Proof.
+Admitted.
+
+Lemma le_add :
+  forall n n' m m' : conat,
+    le n n' -> le m m' -> le (add n m) (add n' m').
+Proof.
+Admitted.
+
+Lemma le_succ_r :
+  forall n m : conat, le n m -> le n (succ m).
+Proof.
+Admitted.
+
+Lemma le_succ :
+  forall n m : conat, le n m -> le (succ n) (succ m).
+Proof.
+Admitted.
+
+
+
+
+
+CoFixpoint sub (n m : conat) : conat :=
+{|
+    pred :=
+      match pred n, pred m with
+          | _, None => pred n
+          | None, _ => None
+          | Some n', Some m' => Some (sub n' m')
+      end;
+|}.
